wip

examples/map/MapA.v
@@ -36,6 +36,7 @@ Section A.
 
   Definition initF: list val -> itree Es val :=
     fun varg =>
+      ;;;
       Ret Vundef
   .
 
@@ -43,21 +44,21 @@ Section A.
     fun varg =>
       '(k, v) <- (pargs [Tint; Tint] varg)?;;;
       f <- pget;;
-      pput (fun n => if Z.eq_dec n k then v else f n);;;
+      _ <- pput (fun n => if Z.eq_dec n k then v else f n);;;
       Ret Vundef
   .
 
   Definition getF: list val -> itree Es val :=
     fun varg =>
       k <- (pargs [Tint] varg)?;;;
-      f <- pget;;
+      f <- pget;;;
       Ret (Vint (f k))
   .
 
   Definition set_by_userF: list val -> itree Es val :=
     fun varg =>
       k <- (pargs [Tint] varg)?;;
-      v <- trigger (Syscall "input" (([]: list Z)↑) (fun _ => True));; v <- v↓?;;
+      v <- trigger (Syscall "input" (([]: list Z)↑) (fun _ => True));; v <- v↓?;;;
       ccallU "set" [Vint v]
   .
 
@@ -70,7 +71,7 @@ Section A.
   Definition SMapSem: SModSem.t := {|
     SModSem.fnsems := MapSbtb;
     SModSem.mn := "Map";
-    SModSem.initial_mr := ε;
+    SModSem.initial_mr := GRA.embed (Excl.unit, Auth.excl ((fun _ => Excl.just 0%Z): @URA.car (nat ==> (Excl.t Z))%ra) ((fun _ => Excl.just 0%Z): @URA.car (nat ==> (Excl.t Z))%ra));
     SModSem.initial_st := (fun (_: Z) => 0%Z)↑;
   |}
   .
